Splinter/Betree/LinkedBranchRefinemment.i.dfy
@@ -1,0 +1,146 @@
+// Copyright 2018-2021 VMware, Inc., Microsoft Inc., Carnegie Mellon University, ETH Zurich, and University of Washington
+// SPDX-License-Identifier: BSD-2-Clause
+ 
+include "LinkedBranch.i.dfy"
+
+// LinkedBranch module stores each node in the b+tree on a different disk address
+
+module LinkedBranchRefinement {
+  import opened Maps
+  import opened Options
+  import opened KeyType
+  import opened ValueMessage
+  import opened Sequences
+  import opened DomainMod
+  import opened GenericDisk
+  import opened Sets
+  import opened LinkedBranchMod
+  import KeysImpl = Lexicographic_Byte_Order_Impl
+  import Keys = KeysImpl.Ord
+  import P = PivotBranchMod
+
+
+  // Interpretation functions
+  function I(branch: LinkedBranch) : (out: P.Node)
+    requires branch.Acyclic()
+    ensures branch.Root().Index? <==> out.Index?
+    ensures branch.AllKeysInRange() ==> out.WF()
+  {
+    var ranking := branch.TheRanking();
+    var out := ILinkedBranchNode(branch, ranking);
+    assert branch.AllKeysInRange() ==> out.WF() by {
+      if branch.AllKeysInRangeInternal(ranking) {
+        ILinkedBranchNodeWF(branch, ranking);
+      }
+    }
+    out
+  }
+
+  function ILinkedBranchNode(branch: LinkedBranch, ranking: Ranking) : (out: P.Node)
+    requires branch.WF()
+    requires branch.ValidRanking(ranking)
+    ensures branch.Root().Index? <==> out.Index?
+    ensures branch.Root().Index? ==> branch.Root().pivots == out.pivots
+    ensures branch.Root().Index? ==> |branch.Root().children| == |out.children|      
+    decreases branch.GetRank(ranking), 1
+  {
+    var node := branch.Root();
+    if node.Leaf? 
+    then P.Leaf(node.keys, node.msgs)
+    else P.Index(node.pivots, IChildren(branch, ranking))
+  }
+
+  function IChildren(branch: LinkedBranch, ranking: Ranking) : (out: seq<P.Node>)
+    requires branch.WF()
+    requires branch.Root().Index?
+    requires branch.ValidRanking(ranking)
+    decreases branch.GetRank(ranking), 0
+  {
+    var numChildren := |branch.Root().children|;
+    seq(numChildren, i requires 0 <= i < numChildren => 
+      ILinkedBranchNode(branch.ChildAtIdx(i), ranking))
+  }
+
+  lemma AllKeysIsConsistentWithI(branch: LinkedBranch, ranking: Ranking)
+    requires branch.WF()
+    requires branch.ValidRanking(ranking)
+    ensures branch.AllKeys(ranking) == ILinkedBranchNode(branch, ranking).AllKeys()
+    decreases branch.GetRank(ranking)
+  {
+    var node := branch.Root();
+    if node.Leaf? {
+    } else {
+      var node' := ILinkedBranchNode(branch, ranking);
+      assert IChildren(branch, ranking) == node'.children; // trigger
+
+      forall k 
+        ensures k in node'.AllKeys() <==> k in branch.AllKeys(ranking)
+      {
+        if k in node'.AllKeys() {
+          if k !in node'.pivots {
+            var i :| 0 <= i < |node'.children| && k in node'.children[i].AllKeys();
+            AllKeysIsConsistentWithI(branch.ChildAtIdx(i), ranking);
+            assert k in branch.AllKeys(ranking);
+          }
+        } else if k in branch.AllKeys(ranking) {
+          if k !in node.pivots {
+            var i :| 0 <= i < |node.children| && k in branch.ChildAtIdx(i).AllKeys(ranking);
+            var linked_child := branch.ChildAtIdx(i);
+            assert ILinkedBranchNode(linked_child, ranking) == node'.children[i];
+            AllKeysIsConsistentWithI(linked_child, ranking);
+            assert k in node'.AllKeys();
+            assert false;
+          }
+        }
+      }
+    }
+  }
+
+  lemma ILinkedBranchNodeWF(branch: LinkedBranch, ranking: Ranking)
+    requires ILinkedBranchNode.requires(branch, ranking)
+    requires branch.AllKeysInRangeInternal(ranking)
+    ensures ILinkedBranchNode(branch, ranking).WF()
+    decreases branch.GetRank(ranking)
+  {
+    var node := branch.Root();
+    var out := ILinkedBranchNode(branch, ranking);
+      
+    if node.Index? {
+      assert |out.pivots| == |out.children| - 1;
+      assert Keys.IsStrictlySorted(out.pivots);
+
+      forall i | 0 <= i < |IChildren(branch, ranking)|
+        ensures IChildren(branch, ranking)[i].WF()
+      {
+        ILinkedBranchNodeWF(branch.ChildAtIdx(i), ranking);
+      }
+
+      assert IChildren(branch, ranking) == out.children; // trigger
+      assert (forall i :: 0 <= i < |out.children| ==> out.children[i].WF());
+
+      forall i | 0 <= i < |out.children|
+        ensures i < |out.children|-1  ==> out.AllKeysBelowBound(i)
+        ensures 0 < i ==> out.AllKeysAboveBound(i)
+      {
+        var child := out.children[i];
+        var linked_child := branch.ChildAtIdx(i);
+          
+        if 0 <= i < |out.children|-1 {
+          assert branch.AllKeysBelowBound(i, ranking);
+        }
+
+        if 0 < i < |out.children| {
+          assert branch.AllKeysAboveBound(i, ranking);
+        }
+
+        AllKeysIsConsistentWithI(linked_child, ranking);
+      }
+    }
+  }
+
+  // query refines
+  // I().WF() ==> msg == I().Query(key)
+  // ILinkedBranchNode(ranking).WF() ==> msg == ILinkedBranchNode(ranking).Query(key)
+
+
+}
