Splinter/Betree/PivotBranchRefinement.i.dfy
@@ -1,15 +1,6 @@
 // Copyright 2018-2021 VMware, Inc., Microsoft Inc., Carnegie Mellon University, ETH Zurich, and University of Washington
 // SPDX-License-Identifier: BSD-2-Clause
- 
-// include "../../lib/Base/KeyType.s.dfy"
-// include "../../Spec/Message.s.dfy"
-// include "../../lib/Base/Option.s.dfy"
-// include "../../lib/Base/Maps.i.dfy"
-// include "../../lib/Base/Sequences.i.dfy"
-// include "../../lib/Base/total_order_impl.i.dfy"
 
-// include "Buffer.i.dfy"
-// include "Domain.i.dfy"
 include "PivotBranch.i.dfy"
 
 module PivotBranchRefinement {
